forcing/Stream.v
@@ -14,9 +14,12 @@ Definition sthead {A : Type} (S : stream A) : A := fst (unfoldp _ S).
 Definition sttail {A : Type} (S : stream A) : ⊳ (stream A) := snd (unfoldp _ S).
 
 Definition const_stream {A : Type} (a : A) : stream A :=
-  fixp (fun x => foldp _ (a,x)).
+  fixp (fun x => a ::: x).
 
 Definition iterate {A : Type}: ⊳ (A -> A) -> A -> stream A
   := fun f => fixp (fun g a => a ::: (g ⊙ (f ⊙ nextp _ a))).
 
 Definition nats : stream nat := iterate (nextp _ S) 0.
+
+Definition stmap {A : Type} f (S : stream A) : stream A :=
+  fixp (fun x => f (sthead S) ::: x).
